su.nsk.iae.rpl/src/su/nsk/iae/rpl/invpatterngenerator/FunctionApplication.java
@@ -41,7 +41,7 @@ public class FunctionApplication extends Term {
 	}
 
 	@Override
-	public InnerExtraInvariantFormula replaceStates(Map<String, UpdateStateVariable> substitution) {
+	public PatternFreeInnerFormula replaceStates(Map<String, UpdateStateVariable> substitution) {
 		UpdateStateVariable newState = substitution.getOrDefault(state.getName(), state);
 		return new FunctionApplication(fnParam, newState);
 	}
