su.nsk.iae.rpl/src/su/nsk/iae/rpl/invpatterngenerator/ImplicationLemmaPremise.java
@@ -4,11 +4,13 @@ import java.util.Map;
 
 import su.nsk.iae.rpl.rPL.FunApplication;
 import su.nsk.iae.rpl.rPL.LemmaPremiseFormula;
+import su.nsk.iae.rpl.rPL.PrimaryTerm;
 import su.nsk.iae.rpl.rPL.RPLFactory;
 import su.nsk.iae.rpl.rPL.RegularFormulaParameter;
 import su.nsk.iae.rpl.rPL.UpdateStateVariable;
 
 public class ImplicationLemmaPremise implements LemmaPremise {
+	static String HOL_IMPLICATION = "-->";
 	private final FunctionApplication left;
 	private final LemmaPremise right;
 	public ImplicationLemmaPremise(FunctionApplication left, LemmaPremise right) {
@@ -34,12 +36,21 @@ public class ImplicationLemmaPremise implements LemmaPremise {
 	@Override
 	public LemmaPremiseFormula convertToEObject() {
 		RPLFactory factory = RPLFactory.eINSTANCE;
-		FunApplication left = (FunApplication) this.left.convertToRPLTerm();
+		PrimaryTerm primTerm = (PrimaryTerm) this.left.convertToRPLTerm();
+		FunApplication left = primTerm.getFunApp();
 		LemmaPremiseFormula right = this.right.convertToEObject();
 		LemmaPremiseFormula result = factory.createLemmaPremiseFormula();
 		result.setLeft(left);
 		result.setRight(right);
 		return result;
+	}
+	
+	@Override
+	public String toString() {
+		StringBuilder stringBuilder = new StringBuilder();
+		stringBuilder.append('(').append(left).append(' ').append(HOL_IMPLICATION).append(' ').append(right);
+		stringBuilder.append(')');
+		return stringBuilder.toString();
 	}
 	
 }
