su.nsk.iae.rpl/src/su/nsk/iae/rpl/invpatterngenerator/NumericConstant.java
@@ -33,7 +33,7 @@ public class NumericConstant extends Term {
 	}
 
 	@Override
-	public InnerExtraInvariantFormula replaceStates(Map<String, UpdateStateVariable> substitution) {
+	public PatternFreeInnerFormula replaceStates(Map<String, UpdateStateVariable> substitution) {
 		return this;
 	}
 	
